name route indexed package provider

rocq/theories/TypeSystem/End2EndSafety.v
@@ -1539,6 +1539,17 @@ Proof.
   - exact Hcallee_check.
 Qed.
 
+Definition strict_exact_closure_component_body_route_package_at_provider
+    (env' : global_env) (f_component : fn_def) : Prop :=
+  forall fname args synthetic_body fdef,
+    direct_call_target_expr (fn_body f_component) =
+      Some (fname, args, synthetic_body) ->
+    lookup_fn fname
+      (env_fns (global_env_with_local_bounds env' (fn_bounds f_component))) =
+      Some fdef ->
+    store_safe_synthetic_direct_call_ready_exact_body_call_route_package_at
+      (global_env_with_local_bounds env' (fn_bounds f_component)) fname.
+
 Lemma infer_program_env_end2end_strict_exact_closure_component_body_exact_body_route_package_at_of_component_check :
   forall env env' f_component fname args synthetic_body fdef,
     infer_program_env_end2end_strict_exact_closure env = infer_ok env' ->
@@ -1786,14 +1797,8 @@ Lemma infer_program_env_end2end_strict_exact_closure_component_body_route_packag
     In f_component (env_fns env') ->
     check_fn_root_shadow_no_capture_direct_call_component_store_safe_summary
       env' f_component = true ->
-    (forall fname args synthetic_body fdef,
-      direct_call_target_expr (fn_body f_component) =
-        Some (fname, args, synthetic_body) ->
-      lookup_fn fname
-        (env_fns (global_env_with_local_bounds env' (fn_bounds f_component))) =
-        Some fdef ->
-      store_safe_synthetic_direct_call_ready_exact_body_call_route_package_at
-        (global_env_with_local_bounds env' (fn_bounds f_component)) fname) /\
+    strict_exact_closure_component_body_route_package_at_provider
+      env' f_component /\
     ((forall fname args synthetic_body,
       direct_call_target_expr (fn_body f_component) =
         Some (fname, args, synthetic_body) ->
